\begin{figure}[H]
\flushleft \shadebox{$\sigma, e \tarrow \sigma$}
\begin{smathpar}
   \inferrule*[lab={\ruleName{$\tarrow$-var-elim}}]
   {
      \sigma, e \tarrow \sigma'
   }
   {
      x \mapsto \sigma, e \tarrow x \mapsto \sigma'
   }
   %
   \and
   %
   \inferrule*[lab={\ruleName{$\tarrow$-var-expr}}]
   {
      \strut
   }
   {
      x \mapsto e, e' \tarrow x \mapsto e
   }
   %
   \and
   %
   \inferrule*[lab={\ruleName{$\tarrow$-true}}]
   {
      \strut
   }
   {
      \{{\exTrue \mapsto \kappa}\}, e \tarrow \{{\exTrue \mapsto \kappa, \exFalse \mapsto e}\}
   }
   %
   \and
   \inferrule*[lab={\ruleName{$\tarrow$-false}}]
   {
      \strut
   }
   {
      \{{\exFalse \mapsto \kappa}\}, e \tarrow \{{\exTrue \mapsto e, \exFalse \mapsto \kappa}\}
   }
   %
   \and
   %
   \inferrule*[lab={\ruleName{$\tarrow$-cons}}]
   {
      \sigma, e \tarrow \sigma'
   }
   {
      \{{\kw{Cons} \ \sigma}\}, e \tarrow \{{\kw{Nil} \mapsto e, \kw{Cons} \ \sigma'}\}
   }
   %
   \and
   %
   \inferrule*[lab={\ruleName{$\tarrow$-nil}}]
   {
      \strut
   }
   {
      \{{\kw{Nil} \mapsto \kappa}\}, e \tarrow \{{\kw{Nil} \mapsto \kappa, \kw{Cons} \ (x \mapsto xs \mapsto e)}\}
   }
   %
   \and
   %
   \inferrule*[lab={\ruleName{$\tarrow$-pair}}]
   {
      \sigma, e \tarrow \sigma'
   }
   {
      \langle \sigma \rangle, e \tarrow \langle \sigma' \rangle
   }
\end{smathpar}
\caption{Totalizing Eliminators}
\end{figure}