\begin{figure}
\flushleft \shadebox{$\sigma \join_{\bullet} \sigma'$}
{\small
\begin{align*}
\elimEmpty \join_{\bullet} \sigma
&=
\sigma
\\
\sigma \join_{\bullet} \elimEmpty
&=
\sigma
\\
(\elimVar{x}{a}) \join_{\bullet} \sigma
&=
\begin{cases}
\elimVar{x}{a \bullet a'}
& \text{if }\sigma = \elimVar{x}{a'}
\\
\elimVar{x}{a}
& \text{otherwise}
\end{cases}
\\
\sigma \join_{\bullet} (\elimVar{x}{a})
&=
\begin{cases}
\elimVar{x}{a \bullet a'}
& \text{if }\sigma = \elimVar{x}{a'}
\\
\elimVar{x}{a}
& \text{otherwise}
\end{cases}
\\
(\elimUnit{a}) \join_{\bullet} (\elimUnit{a'})
&=
\elimUnit{a \bullet a'}
\\
\elimSum{\sigma}{\tau} \join_{\bullet} \elimSum{\sigma'}{\tau'}
&=
\elimSum{\sigma \join_{\bullet} \sigma'}{\tau \join_{\bullet} \tau'}
\\
\elimProd{\sigma} \join_{\bullet} \elimProd{\sigma'}
&=
\elimProd{\sigma \join_{\join_{\bullet}} \sigma'}
\\
(\elimRoll{\sigma}) \join_{\bullet} (\elimRoll{\sigma'})
&=
\elimRoll{(\sigma \join_{\bullet} \sigma')}
\\
(\elimFun{a}) \join_{\bullet} (\elimFun{a'})
&=
\elimFun{a \bullet a'}
\end{align*}}
\caption{Joining two eliminators of the same type}
\end{figure}
