\begin{figure}
\flushleft \shadebox{$\sigma \join_{\bullet} \sigma'$}
{\small
\begin{align*}
\trieEmpty \join_{\bullet} \sigma
&=
\sigma
\\
\sigma \join_{\bullet} \trieEmpty
&=
\sigma
\\
(\trieVar{x}{a}) \join_{\bullet} \sigma
&=
\begin{cases}
\trieVar{x}{a \bullet a'}
& \text{if }\sigma = \trieVar{x}{a'}
\\
\trieVar{x}{a}
& \text{otherwise}
\end{cases}
\\
\sigma \join_{\bullet} (\trieVar{x}{a})
&=
\begin{cases}
\trieVar{x}{a \bullet a'}
& \text{if }\sigma = \trieVar{x}{a'}
\\
\trieVar{x}{a}
& \text{otherwise}
\end{cases}
\\
(\trieUnit{a}) \join_{\bullet} (\trieUnit{a'})
&=
\trieUnit{a \bullet a'}
\\
\trieSum{\sigma}{\tau} \join_{\bullet} \trieSum{\sigma'}{\tau'}
&=
\trieSum{\sigma \join_{\bullet} \sigma'}{\tau \join_{\bullet} \tau'}
\\
\trieProd{\sigma} \join_{\bullet} \trieProd{\sigma'}
&=
\trieProd{\sigma \join_{\join_{\bullet}} \sigma'}
\\
(\trieRoll{\sigma}) \join_{\bullet} (\trieRoll{\sigma'})
&=
\trieRoll{(\sigma \join_{\bullet} \sigma')}
\\
(\trieFun{a}) \join_{\bullet} (\trieFun{a'})
&=
\trieFun{a \bullet a'}
\end{align*}}
\caption{Joining two tries of the same type}
\end{figure}
